Got compcert primitives to compute, with Gregory's help. Should be able to start doing interesting proofs about controllers now with the abstractor.

compile/source.v
@@ -42,8 +42,12 @@ Hypothesis precThm : forall k : ,Z
      k - Fcore_FLT.FLT_exp (3 - emax - prec) prec k)%Z.*)
 
 Definition prec:Z := 24%Z.
-Definition emax:Z := 128%Z.
-Definition emin:Z := (3 - emax - prec)%Z.
+(* Definition emax:Z := 128%Z.
+   Definition emax:Z := 1023%Z. *)
+Definition emax := 128%Z.
+
+(*Definition emin:Z := (3 - emax - prec)%Z.*)
+Definition emin:Z := (-126)%Z.
 Definition emaxGtEmin : (emax > emin)%Z.
 Proof. compute. reflexivity.
 Defined.
@@ -74,11 +78,8 @@ Proof.
   - rewrite Z.compare_lt_iff in Hk.
     unfold emin, emax, prec in *.
     simpl in *.
-
-    (* WARNING WARNING WARNING
-       As stated, with these constants, this theorem is not true!
-       WARNING WARNING WARNING *)
-Admitted.    
+    psatz Z.
+Qed.
 
 Definition custom_prec := prec.
 Definition custom_emax:= emax.
@@ -98,12 +99,6 @@ Proof.
 unfold custom_emax,custom_emin.
 apply emaxGtEmin.
 Qed.
-Print Floats.float.
-Print binary64.
-Print binary_float.
-
-SearchAbout binary_float.
-Locate Fappli_IEEE_extra.Beq_dec.
 
 (* Term, sans the next operator *)
 Inductive NowTerm : Type :=
@@ -159,8 +154,6 @@ Coercion nat_to_int : nat >-> int.
 
 Coercion Pos.of_nat : nat >-> positive.
 (*Coercion FloatToR : Floats.float >-> R.*)
-
-Print binary_float.
 
 (* inject  *)
 Fixpoint denowify (nt : NowTerm) : Term :=
@@ -312,21 +305,90 @@ Definition lift2 {T U V : Type} (f : T -> U -> V) (a : option T) (b : option U) 
   | _ , _ => None
   end.
 
+(* Useful floating-point operations for our format *)
+Definition float_plus (a b : float) : float :=
+  Bplus custom_prec custom_emax custom_precGt0 custom_precLtEmax custom_nan mode_NE a b.
+
+Definition float_minus (a b : float) : float :=
+  Bminus custom_prec custom_emax custom_precGt0 custom_precLtEmax custom_nan mode_NE a b.
+
+Definition float_mult (a b : float) : float :=
+  Bmult custom_prec custom_emax custom_precGt0 custom_precLtEmax custom_nan mode_NE a b.
+
+(* This replaces a validity proof in the floating-point representation and replaces it with
+   eq_refl (this is possible since boolean equality is decidable). Doing this optimization
+   allows us to compute floating-point operations in Coq, (including constructing
+   floating-point numbers) though we must do so using lazy. *)
+Definition concretize_float (f : float) :=
+  match f with
+  | B754_finite sig m e pf =>
+    @B754_finite _ _ sig m e
+                (match bounded prec emax m e as X return (X = true -> X = true) with
+                 | true => fun p => eq_refl
+                 | false => fun p => p
+                 end pf)
+  | _ => f
+  end.
+
+Lemma concretize_float_correct :
+  forall (f : float), concretize_float f = f.
+Proof.
+  intros.
+  unfold concretize_float.
+  destruct f; try reflexivity.
+  assert (((if bounded prec emax m e as X return (X = true -> X = true)
+       then fun _ : true = true => eq_refl
+            else fun p : false = true => p) e0) = e0).
+  { unfold custom_prec, custom_emax in e0.
+    rewrite e0. reflexivity. }
+  rewrite H. reflexivity.
+Qed.
+
+(* here is how we define new floating-point constants. *)
+Definition new_float_one := Eval lazy in (concretize_float (nat_to_float 1)).
+
+(* raw representaion of float 1 as bits (obtained from simple C program) *)
+Lemma test : new_float_one = concretize_float (b32_of_bits 1065353216).
+Proof.
+  unfold new_float_one.
+  unfold b32_of_bits.
+  unfold binary_float_of_bits.
+  lazy.
+  reflexivity.
+Qed.
+
+(* and here is how we add them *)
+Definition new_float_one' := Eval lazy in (concretize_float (float_plus custom_float_zero (nat_to_float 1))).
+
+(* These examples illustrate how "concretize_float" should be used: you should wrap an entire float-typed expression in it
+   and then run Eval lazy. "Concretize_float" is an aid to evaluation, essentially. *)
+
+(* Floating-point comparisons *)
+(* NB: sign bit is true if negative *)
+Definition float_lt (a b : float) : bool :=
+  match float_minus a b with
+  | B754_zero _ => false
+  | B754_infinity is_neg => is_neg
+  | B754_nan is_neg _ => is_neg (* should never happen for non-exceptional operands... *)
+  | B754_finite is_neg _ _ _ => is_neg
+  end.
+
+Definition float_le (a b : float) : bool :=
+  match float_minus a b with
+  | B754_zero _ => true
+  | B754_infinity is_neg => is_neg
+  | B754_nan is_neg _ => is_neg (* should never happen for non-exceptional operands... *)
+  | B754_finite is_neg _ _ _ => is_neg
+  end.  
 
 Section eval_expr.
   Variable st : fstate.
 
   (* denotation of NowTerm *)
-  Print Floats.Float.binop_pl.
-  
-  Print Floats.Float.transform_quiet_pl.
 
-  Print Archi.default_pl_64.
-
+  (* TODO - does this actually get used anywhere? --M *)
 Definition try := (fun pl : positive =>
    ((PreOmega.Z_of_nat' (S (Fcore_digits.digits2_Pnat pl)) <? 53)%Z = true)%type).
-
-Print Bplus.
 
 Fixpoint eval_NowTerm (t:NowTerm) :=
   match t with
@@ -334,19 +396,17 @@ Fixpoint eval_NowTerm (t:NowTerm) :=
   | NatN n => Some (nat_to_float n)
   | FloatN f => Some f
   | PlusN t1 t2 =>
-    lift2 (Bplus custom_prec custom_emax custom_precGt0 custom_precLtEmax custom_nan mode_NE)
+    lift2 float_plus
           (eval_NowTerm t1) (eval_NowTerm t2)
   | MinusN t1 t2 =>
-    lift2 (Bminus custom_prec custom_emax custom_precGt0 custom_precLtEmax custom_nan mode_NE)
+    lift2 float_minus
           (eval_NowTerm t1) (eval_NowTerm t2)
   | MultN t1 t2 =>
-    lift2 (Bmult custom_prec custom_emax custom_precGt0 custom_precLtEmax custom_nan mode_NE)
+    lift2 float_mult
           (eval_NowTerm t1) (eval_NowTerm t2)
   end.
 
   (* denotation of comparison functions *)
-
-
 
 Definition custom_cmp (c : comparison) (f1 : float) (f2 : float) := Floats.cmp_of_comparison c (Fappli_IEEE_extra.Bcompare custom_prec custom_emax f1 f2).
 
@@ -396,9 +456,6 @@ Fixpoint assns_update_state (assns: list progr_assn) (acc : fstate) : option fst
   end.
 *)
 
-Print SrcProg.
-SearchAbout FlatFormula.
-
 Fixpoint eval_SrcProg (sp : SrcProg) (init : fstate) : option fstate :=
   match sp with
     | SAssn v nt   => assn_update_state v nt init
@@ -415,18 +472,6 @@ Fixpoint eval_SrcProg (sp : SrcProg) (init : fstate) : option fstate :=
         | None       => None
       end
   end.
-
-Locate custom_float_zero.
-Locate Zdigits2.
-
-Extraction "deps.ml" nat_to_float.
-
-Extraction nat_to_float.
-
-Print nat_to_float.
-Print Fappli_IEEE_extra.BofZ.
-Print binary_normalize.
-Print FF2B.
 
 (* failed effort to get nat_to_float to compute *)
 (*
@@ -494,3 +539,4 @@ Fixpoint eval_progr (p : progr) (init : fstate) : option fstate :=
     end
   end.
 *)
+
